qtesla/code/params-I/Hacl.Impl.QTesla.Pack.fst
@@ -28,8 +28,10 @@ module LL = Lib.Loops
 
 open Hacl.Impl.QTesla.Params
 open Hacl.Impl.QTesla.Globals
+open Hacl.Impl.QTesla.ShiftArithmeticLeft
+module SP = QTesla.Params
 
-#reset-options "--z3rlimit 500 --max_fuel 1 --max_ifuel 1"
+#reset-options "--z3rlimit 300 --max_fuel 0 --max_ifuel 0"
 
 private inline_for_extraction noextract
 val encode_sk_s:
@@ -102,56 +104,40 @@ let encode_or_pack_sk = encode_sk
 
 private inline_for_extraction noextract
 val decode_sk_s:
-    j : size_t//{v j + 5 * v params_n <= v crypto_secretkeybytes}
+    j_in : size_t{v j_in + 5 * v params_n < v crypto_secretkeybytes}
   -> s : lbuffer I16.t params_n
   -> sk : lbuffer uint8 crypto_secretkeybytes
   -> Stack size_t
     (requires fun h -> live h s /\ live h sk /\ disjoint s sk)
-    (ensures fun h0 _ h1 -> modifies1 s h0 h1 /\ is_s_sk h1 s)
+    (ensures fun h0 r h1 -> modifies1 s h0 h1 /\ is_s_sk h1 s /\ r = v j_in + (v params_n `FStar.Int.op_Slash` 4) * 5)
 
-#reset-options "--z3rlimit 1000 --max_fuel 1 --max_ifuel 1 --admit_smt_queries true"
-
-let decode_sk_s j s sk =
-    push_frame();
-    let iBuf = create (size 1) (size 0) in
-    let jBuf = create (size 1) j in
-
+let decode_sk_s j_in s sk =
     let h0 = ST.get () in
-    LL.while
-    (fun h -> live h s /\ live h sk /\ live h iBuf /\ live h jBuf /\ modifies3 s iBuf jBuf h0 h)// /\ 
-           //v (bget h jBuf 0) + 4 < v crypto_secretkeybytes) // Can't prove this yet. Assumed below.
-    (fun h -> v (bget h iBuf 0) < v params_n)
-    (fun _ -> iBuf.(size 0) <. params_n)
-    (fun _ ->
-        let i = iBuf.(size 0) in
-	let j = jBuf.(size 0) in
+    for 0ul (params_n /. size 4)
+    (fun h _ -> live h s /\ live h sk /\ modifies1 s h0 h)
+    (fun k ->
+        let i = k *. size 4 in
+	let j = j_in +. k *. size 5 in
 
-        //assert_norm(v params_n / 5 < v crypto_secretkeybytes);
-        assume(v j + 4 < v crypto_secretkeybytes);
         let skj0 = sk.(j+.size 0) in    [@inline_let] let skj0 = Lib.RawIntTypes.u8_to_UInt8 skj0 in    
         let skj1 = sk.(j+.size 1) in    [@inline_let] let skj1 = Lib.RawIntTypes.u8_to_UInt8 skj1 in
 	let skj2 = sk.(j+.size 2) in    [@inline_let] let skj2 = Lib.RawIntTypes.u8_to_UInt8 skj2 in    
         let skj3 = sk.(j+.size 3) in    [@inline_let] let skj3 = Lib.RawIntTypes.u8_to_UInt8 skj3 in
 	let skj4 = sk.(j+.size 4) in    [@inline_let] let skj4 = Lib.RawIntTypes.u8_to_UInt8 skj4 in
 
-        assume(v i + 3 < v params_n);
-        s.(i+.size 0) <- I16.(uint8_to_int16 skj0               |^ int32_to_int16 I32.(((uint8_to_int32 skj1) <<^ 30ul) >>>^ 22ul));
-	s.(i+.size 1) <- I16.(uint8_to_int16 UI8.(skj1 >>^ 2ul) |^ int32_to_int16 I32.(((uint8_to_int32 skj2) <<^ 28ul) >>>^ 22ul));
-	s.(i+.size 2) <- I16.(uint8_to_int16 UI8.(skj2 >>^ 4ul) |^ int32_to_int16 I32.(((uint8_to_int32 skj3) <<^ 26ul) >>>^ 22ul));
-        //assert(UI8.v skj4 >= 0);
-        //assert(I8.v (uint8_to_int8 skj4) >= 0);
-        assume(I16.v (int8_to_int16 (uint8_to_int8 skj4)) >= 0);
-	s.(i+.size 3) <- I16.(uint8_to_int16 UI8.(skj3 >>^ 6ul) |^ (int8_to_int16 (uint8_to_int8 skj4)) <<^ 2ul);
+        [@inline_let] let (<<<^) = shift_arithmetic_left_i32 in
+        
+        s.(i+.size 0) <- I16.(uint8_to_int16 skj0               |^ int32_to_int16 I32.(((uint8_to_int32 skj1) <<<^ 30ul) >>>^ 22ul));
+	s.(i+.size 1) <- I16.(uint8_to_int16 UI8.(skj1 >>^ 2ul) |^ int32_to_int16 I32.(((uint8_to_int32 skj2) <<<^ 28ul) >>>^ 22ul));
+	s.(i+.size 2) <- I16.(uint8_to_int16 UI8.(skj2 >>^ 4ul) |^ int32_to_int16 I32.(((uint8_to_int32 skj3) <<<^ 26ul) >>>^ 22ul));
+        [@inline_let] let (<<<^) = shift_arithmetic_left_i16 in
 
-        jBuf.(size 0) <- j +. size 5;
-	iBuf.(size 0) <- i +. size 4
+	s.(i+.size 3) <- I16.(uint8_to_int16 UI8.(skj3 >>^ 6ul) |^ (int8_to_int16 (uint8_to_int8 skj4)) <<<^ 2ul)
     );
 
-    let j = jBuf.(size 0) in
-    pop_frame();
     let hReturn = ST.get () in
     assume(is_s_sk hReturn s);
-    j
+    j_in +. (params_n /. size 4) *. size 5
 
 val decode_sk:
     seeds : lbuffer uint8 (size 2 *. crypto_seedbytes)
@@ -164,22 +150,22 @@ val decode_sk:
 		    disjoint s e /\ disjoint s sk /\ disjoint e sk)
     (ensures fun h0 _ h1 -> modifies3 seeds s e h0 h1 /\ is_s_sk h1 s /\ is_e_sk h1 e)
 
+//#push-options "--initial_fuel 1 --max_fuel 1"
 let decode_sk seeds s e sk =
-    push_frame();
     let h0 = ST.get () in
+    assume(0 + 5 * SP.params_n < v crypto_secretkeybytes);
     let j = decode_sk_s (size 0) s sk in
     let h1 = ST.get () in
     assert(modifies1 s h0 h1);
     let _ = decode_sk_s j e sk in
     let h2 = ST.get () in
     assert(modifies2 s e h0 h2);
-    assume(v (size 2 *. params_s_bits *. params_n /. size 8) + v (size 2 *. crypto_seedbytes) < v crypto_secretkeybytes);
+    assert_norm(v (size 2 *. params_s_bits *. params_n /. size 8) + v (size 2 *. crypto_seedbytes) < v crypto_secretkeybytes);
     copy seeds (sub sk (size 2 *. params_s_bits *. params_n /. size 8) (size 2 *. crypto_seedbytes));  
 
     let h3 = ST.get () in
-    assert(modifies3 s e seeds h0 h3);
-
-    pop_frame()
+    assert(modifies3 s e seeds h0 h3)
+//#pop-options
 
 // These four functions have the same implementation as III-size, so we share its code.
 inline_for_extraction noextract
